More work in coq/Extensible.v

coq/Extensible.v
@@ -672,6 +672,124 @@ Program Fixpoint refine {s s' a} (AbsR : s -> s' -> Prop)
     end
   end.
 
+Class Refines (eff : Type -> Type) := {
+  refinement : forall a, eff a -> a -> Prop;
+  candidate  : forall a (e : eff a), { x | refinement _ e x }
+}.
+
+Arguments refinement {eff _ a} _ _.
+Arguments candidate {eff _ a} _.
+
+Fixpoint refineG {effs effs' a}
+         (n : nat)
+         (all_refinable : forall eff,
+             In eff effs + In eff effs' -> Refines eff)
+         (old : Eff effs a) (new : Eff effs' a) : Prop.
+Proof.
+  destruct n.
+    exact False.
+  destruct old, new.
+  - exact (a0 = a1).
+  - induction effs'; [now inversion u|].
+    inversion u; subst; clear u.
+      pose proof (all_refinable a1 (inr (in_eq _ _))).
+      exact (refineG _ _ _ n all_refinable (Pure a0) (f (` (candidate X)))).
+    apply IHeffs'; intuition.
+    exact (Pure a0).
+  - induction effs; [now inversion u|].
+    inversion u; subst; clear u.
+      pose proof (all_refinable a1 (inl (in_eq _ _))).
+      exact (refineG _ _ _ n all_refinable (f (` (candidate X))) (Pure a0)).
+    apply IHeffs; intuition.
+    exact (Pure a0).
+  - induction effs;  [now inversion u|].
+    induction effs'; [now inversion u0|].
+    inversion u; subst; clear u.
+      pose proof (all_refinable a0 (inl (in_eq _ _))).
+      inversion u0; subst; clear u0.
+        pose proof (all_refinable a1 (inr (in_eq _ _))).
+        exact (refineG _ _ _ n all_refinable
+                       (f (` (candidate X))) (f0 (` (candidate X1)))).
+      apply IHeffs'; intuition; intros.
+      admit.
+    eapply IHeffs; intuition; intros.
+    admit.
+Admitted.
+
+Program Fixpoint refineG {effs effs' a} (n : nat)
+        (old : Eff effs a) (new : Eff effs' a) : Prop :=
+  match n with
+  | O => False
+  | S n' =>
+    match old, new with
+    | Pure x, Pure y => x = y
+
+    | Pure x, Impure u k =>
+      match effs' with
+      | nil => !
+      | _ :: _ =>
+        match decomp u with
+        | inl (Pick P) => exists v, P v /\ refineG n' old (k v)
+        | inr u' =>
+          match decomp u' with
+          | inl f => exists s,
+                     refineG n' old (k (_ (snd (State_func f s))))
+          | inr u' => !
+          end
+        end
+      end
+
+    | Impure u k, Pure y =>
+      match effs' with
+      | nil => !
+      | _ :: _ =>
+        match decomp u with
+        | inl (Pick P) => exists v, P v /\ refineG n' (k v) new
+        | inr u' =>
+          match decomp u' with
+          | inl f => exists s,
+                     refineG n' (k (_ (snd (State_func f s)))) new
+          | inr u' => !
+          end
+        end
+      end
+
+    | Impure xu xk, Impure yu yk =>
+      match effs, effs' with
+      | nil, _ => !
+      | _, nil => !
+      | _ :: _, _ :: _ =>
+        match decomp xu, decomp yu with
+        | inl f, inl g => refineChoice f (_ g)
+
+        | inl (Pick P), inr yu' =>
+          match decomp yu' with
+          | inl g => exists v s,
+                     P v /\ refineG n' (xk v) (yk (_ (snd (State_func g s))))
+          | inr u' => !
+          end
+
+        | inr xu', inl (Pick P) =>
+          match decomp xu' with
+          | inl f => exists v s,
+                     P v /\ refineG n' (xk (_ (snd (State_func f s)))) (yk v)
+          | inr u' => !
+          end
+
+        | inr xu', inr yu' =>
+          match decomp xu', decomp yu' with
+          | inl f, inl g => exists s s', s s' ->
+                                         refineG n' (xk (_ (snd (State_func f s))))
+                                                 (yk (_ (snd (State_func g s'))))
+          | inl _,   inr yu' => !
+          | inr xu', inl _   => !
+          | inr xu', inr _   => !
+          end
+        end
+      end
+    end
+  end.
+
 (* This is supposed to be the effect handler for non-deterministic choice,
    which simply denotes the choice as a propositional relation in Gallina over
    the remaining effects to be handled. *)
